\documentclass{article}
\usepackage{header}
%%%%%%%%%%%%%%%%%%%%%%%%%%%%%%%%%%%%%%%%%%%%%%%%%%%%%%%%
%Preamble

\title{Standard Model Notes}
\author{Linden Disney-Hogg}
\date{January 2019}

%%%%%%%%%%%%%%%%%%%%%%%%%%%%%%%%%%%%%%%%%%%%%%%%%%%%%%%%
%%%%%%%%%%%%%%%%%%%%%%%%%%%%%%%%%%%%%%%%%%%%%%%%%%%%%%%%
\begin{document}

\maketitle
\tableofcontents

\section{Introduction}
The Standard Model (SM) describes three fundamental forces (EM, weak, and strong). The forces are mediated by gauge bosons (spin $=1$).
\begin{itemize}
    \item EM (QED) : photon $\gamma$, (massless)
    \item Weak : $W$ and $Z$ bosons
    \item Strong : gluons $g$ (massless)
\end{itemize}
Matter content (spin $-\frac{1}{2}$ fermions) comes in three generations 
\begin{itemize}
    \item Neutrinos  $\nu_e, \nu_\mu \nu_\tau$ weak 
    \item Charged leptons $e, \mu, \tau$ weak and EM
    \item Quarks $u,d c,s,t,b$, weak, EM, and strong. 
\end{itemize}
There is also the Higgs boson $H$ (scalar, spin 0), responsible for generating the mass of W and Z bosons. 

Gauge bosons are manifestations of local symmetries. In SM the gauge group is 
\[
\underbrace{SU(3)_c}_{\text{color}} \times \underbrace{SU(2)_L}_{\text{chiral left}} \times \underbrace{U(1)_\gamma}_{\text{hypercharge}}
\]

%%%%%%%%%%%%%%%%%%%%%%%%%%%%%%%%%%%%%%%%%%%%%%%%%%%%%%%%
%%%%%%%%%%%%%%%%%%%%%%%%%%%%%%%%%%%%%%%%%%%%%%%%%%%%%%%%
\section{Chiral and Gauge symmetries}
%%%%%%%%%%%%%%%%%%%%%%%%%%%%%%%%%%%%%%%%%%%%%%%%%%%%%%%%
\subsection{Chiral symmetry}

Spin 1/2 particles are Dirac fermions with spinor field $\psi$ that satisfy the Dirac equation $(i\slashed{\del}-m)\psi=0$. The Dirac adjoint $\bar{\psi} = \psi^\dagger \gamma^0$ satisfies $\bar{\psi}(i\slashed{\del}^\leftarrow - m)=0$ where $\slashed{\del}^\leftarrow$ acts to the left. Dirac matrices satisfy 
\[
\acomm[\gamma^\mu]{\gamma^\nu}=2g^{\mu\nu}I
\]
where $g^{\mu\nu}=\diag(1,-1,-1,-1)$. Also define 
\[
\gamma^5 = i \gamma^0 \gamma^1 \gamma^2 \gamma^3
\]
which satisfies $(\gamma^5)^2=I$ and $\acomm[\gamma^\mu]{\gamma^5}=0$. In general the \emph{Chiral} or \emph{Weyl} basis is used, where 
\begin{align*}
    \gamma^0 &= \begin{pmatrix} 0 & I_2 \\ I_2 & 0 \end{pmatrix} \\
    \gamma^i &= \begin{pmatrix} 0 & \sigma_i \\ -\sigma_i & 0 \end{pmatrix} \\ 
\end{align*}
In this representation 
\[
\gamma^5=\begin{pmatrix} -I_2 & 0 \\ 0 & I_2 \end{pmatrix}
\]
Consider the massless limit of the Dirac equation
\[
\slashed{\del}\psi = 0 \Rightarrow \slashed{\del} ( \gamma^5\psi) = 0. 
\]
Define $P_{R,L}=\frac{1}{2} (1 \pm \gamma^5)$, projection operators. Then correspondingly let $\psi_{R,L} = P_{R,L} \psi$. Then $\gamma^5 \psi_{R,L} = \pm \psi_{R,L}$, so the projections are eigenstates of chirality. In the chiral basis, $\psi_{R,L}$ only contain lower/upper 2-component spinor degrees of freedom (d.o.f). As a result $\psi_{R,L}$ annihilates left/right handed chiral particles respectively. In addition 
\[
\bar{\psi}_{R,L} = (P_{R,L} \psi)^\dagger \gamma^0 = \psi^\dagger \frac{1}{2} (1\pm\gamma^5)\gamma^0=\bar{\psi} P_{L,R}
\]
A massless Dirac fermion has a \emph{global} $U(1)_L \times U(1)_R$ chiral symmetry. Under $U(1)_{R,L}$, $\psi_{R,L} \mapsto e^{i\alpha_{R,L}} \psi_{R,L}$, as can be seen from the Dirac Lagrangian 
\[
\mc{L}_D = \bar{\psi}(i\slashed{\del}-m)\psi = \bar{\psi}_L i \slashed{\del} \psi_L + \bar{\psi}_R i \slashed{\del} \psi_R - m(\bar{\psi}_R\psi_L + \bar{\psi}_L \psi_R) 
\]
The mass term explicitly breaks the chiral symmetry to a remaining vector symmetry where $\alpha_L = \alpha_R = \alpha$, so $\psi \mapsto e^{i\alpha} \psi$, $U(1)_L \times U(1)_R \to U(1)_V$. 

%%%%%%%%%%%%%%%%%%%%%%%%%%%%%%%%%%%%%%%%%%%%%%%%%%%%%%%%
\subsection{Review of Dirac Field}
Quantise 
\[
\psi(x) = \sum_{p,s} \left[ b^s(p) u^s(p) e^{-ip\cdot x} + {d^s}^\dagger(p) v^s(p) e^{ip\cdot x} \right]
\]
$s=\pm\frac{1}{2}$, and $\sum_p = \int \LImeas$, $\braket{p|q} = (2\pi)^2 (2E_p)\delta^3(\bm{p}-\bm{q})$ with $\ket{p} = b^\dagger(p) \ket{0}$. $u$ and $v$ are solutions of 
\[
(\slashed{p}-m)u=0 , \quad (\slashed{p}+m)v=0
\]
In the chiral basis these become 
\begin{align*}
    u^s(p) &= \begin{pmatrix} \sqrt{p\cdot \sigma} \xi^s \\ \sqrt{p\cdot\bar{\sigma}} \xi^s \end{pmatrix} \\ 
    v^s(p) &= \begin{pmatrix} \sqrt{p\cdot \sigma} \xi^s \\ -\sqrt{p\cdot\bar{\sigma}} \xi^s \end{pmatrix}
\end{align*}
with $\sigma^\mu = (1, \bm{\sigma})$, $\bar{\sigma}^\mu = (1, -\bm{\sigma})$. 

\begin{definition}[Helicity]
\bam{Helicity} is defined as the projection of angular momentum onto the linear momentum direction. 
\[
h = \bm{J} \cdot \hat{\bm{p}} = \bm{s} \cdot \hat{\bm{p}}
\]
as $\bm{J} = \bm{r}\times\bm{p} + \bm{s}$, and 
\[
s_i = \frac{i}{4}\eps_{ijk} \gamma^i \gamma^j = \frac{1}{2} \begin{pmatrix} \sigma_i & 0 \\ 0 & \sigma_i \end{pmatrix}
\]
\end{definition}
A massless spinor satisfies $\slashed{p}u=0$
so 
\[
hu(p) = \frac{\gamma^5}{2} u(p) 
\]
\[
\Rightarrow hu_{R,L} = \frac{\gamma^5}{2} u_{R,L} = \pm \frac{1}{2} u_{R,L}
\]
Note
\begin{itemize}
     \item Chiral states are only eigenstates of the Dirac equation when $m=0$
     \item Helicity is defined for $m=0$ and $m\neq0$, but it's not Lorentz Invariant when $m\neq 0$. 
     \item There is only a 1-1 correspondence between helicity and chirality when $m=0$. 
\end{itemize}

%%%%%%%%%%%%%%%%%%%%%%%%%%%%%%%%%%%%%%%%%%%%%%%%%%%%%%%%
\subsection{Gauge Symmetry}
Promoting $\alpha$ to a function of $x$, $\alpha(x)$, i.e. gauging the symmetry $\psi \to e^{i\alpha(x)} \psi$, the kinetic term is no longer invariant. 
\[
\bar{\psi} i \slashed{\del} \psi \to \bar{\psi} i \slashed{\del} \psi - (\bar{\psi}\gamma^mu \psi)(\del_\mu \alpha(x))
\]
Introduce a gauge covariant derivative $D_\mu$ such that
\[
D_\mu \psi(x) \to e^{i\alpha(x)} D_\mu \psi(x)
\]
To do this introduce a gauge field $A_\mu(x)$ so 
\[
D_\mu \psi = (\del_\mu + igA_\mu) \psi
\]
where $A_\mu \to A_\mu-\frac{1}{g} \del_\mu \alpha$ so $\bar{\psi} i \slashed{D} \psi$ is invariant. \\
Introduce a kinetic term for the gauge fields 
\begin{align*}
\mc{L}_{gauge} &= -\frac{1}{4} F_{\mu\nu} F^{\mu\nu} \\
F_{\mu\nu} &= \del_\mu A_\nu - \del_\nu A_\mu \\
ig F_{\mu\nu} &= \comm[D_\mu]{D_\nu}
\end{align*}
QED has a $U(1)$ gauge symmetry that treats LH and RH fields equivalently. The weak gauge bosons only couple to LH fields, but $U(1)$ is not the appropriate symmetry, we need $SU(2)$. (We will review non-abelian gauge symmetries later.) 

\subsection{Types of Symmetry}
Symmetries may manifest themselves in a variety of ways: 
\begin{itemize}
    \item Symmetry is intact e.g. $U(1)_{EM}$, and $SU(3)_c$ gauge symmetries. 
    \item Symmetry of $\mc{L}$ is broken by an \bam{anomaly} (holds classically but is broken by quantum loop effects). Not actually a true symmetry. E.g. global axial $U(1)$ symmetry in the SM.
    \item Symmetries can hold for some terms in $\mc{L}$ but not others. This is called "broken explicitly". It may be an approximate symmetry if the breaking terms are small. E.g. global 'isospin' symmetry relating $u$ and $d$ quarks in QCD.
    \item Hidden symmetries - respected by $\mc{L}$ but \emph{not} the vacuum. These can be: a) \bam{spontaneously broken symmetries}, vacuum expectation value from one or more scalar fields non-zero, e.g $SU(2)_L \times U(1)_\gamma \to U(1)_{EM}$, or b) Even without scalar fields get \bam{dynamical breaking} from quantum effects. e.g. $SU(2)_L \times SU(2)_R$ global symmetry in QCD (massless quarks). 
\end{itemize}

%%%%%%%%%%%%%%%%%%%%%%%%%%%%%%%%%%%%%%%%%%%%%%%%%%%%%%%%
%%%%%%%%%%%%%%%%%%%%%%%%%%%%%%%%%%%%%%%%%%%%%%%%%%%%%%%%
\section{Discrete Symmetries}
The discrete symmetries are 
\begin{itemize}
    \item Parity $P : (t,\bm{x}) \to (t,-\bm{x})$
    \item Time reversal $T : (t,\bm{x}) \to (-t,\bm{x})$
    \item Charge conjugation $C : \text{particles} \leftrightarrow \text{antiparticles} $
\end{itemize}
Parity and Time reversal are spacetime symmetries. These have properties such as 
\begin{itemize}
    \item $\bar{\psi}\gamma^\mu \psi$ couplings between gauge bosons and fermions,  e.g. QED and QCD, are invariant under $P$ and $C$ separately.  
    \item $\bar{\psi}\gamma^\mu (1-\gamma^5) \psi$ couplings to fermions, e.g. weak interactions, are not.
    \item Weak interaction violates $CP$, which leads to $T$ violation from the $CPT$ theorem. 
\end{itemize}
We will first investigate the consequences of $C,P,T$ symmetries in order to understand the above statements. 

%%%%%%%%%%%%%%%%%%%%%%%%%%%%%%%%%%%%%%%%%%%%%%%%%%%%%%%%
\subsection{Symmetry Operators} 

\begin{theorem}[Winger]
If physics is invariant under $\Psi \to \Psi^\prime$ (where $\Psi, \Psi^\prime \in \mc{H}$ some Hilbert space), then $\exists W$ an operator such that $\Psi^\prime = W\Psi$ where either W i) linear and unitary or ii) antilinear and antiunitary. 
\end{theorem}
\begin{proof}
Consider a Poincare transform 
\[
x^\mu \to \Lambda^\mu_\nu x^\nu + a^\mu
\]
Then for a parity transform 
\[
\Lambda^\mu_\nu = \mbb{P}^\mu_\nu = \diag(1,-1,-1,-1)
\]
and for time reversal
\[
\mbb{T}^\mu_\nu = \diag(-1,1,1,1)
\]
The corresponding operator can be expanded as 
\[
W(\Lambda,a) = W(1+1,\eps) = 1+\frac{i}{2} w_{\mu\nu} J^{\mu\nu} - i\eps_\mu p^\mu
\]
where the $J$ are the generators of boosts and rotations, and $p$ the generators of translation i.e $p^0=H=$Hamiltonian and $p^i=$momentum. Then
\begin{align*}
    \hat{P} &= W(\mbb{P},0) \\
    \hat{T} &= W(\mbb{T},0)
\end{align*}
Now from general composition rules 
\[
\hat{P} W(\Lambda,a) \hat{P}^{-1} = W(\mbb{P}\Lambda\mbb{P}^{-1},\mbb{P}a)
\]
Insert expansion of $W$ and compare coefficients of $-\eps_0$ to get 
\[
\hat{P} iH \hat{P}^{-1} = iH
\]
and doing likewise for $\hat{T}$ gives 
\be
\hat{T} iH \hat{T}^{-1} = -iH \label{eq:SM:1}
\ee
Suppose $\Psi$ is an energy eigenstate
\[
(\Psi, iH\Psi) = (\Psi, iE\Psi) = iE
\]
If $\hat{P},\hat{T}$ are symmetries then $\hat{P}\Psi,\hat{T}\Psi$ should also be energy eigenstates with the same energy. 
Suppose $\hat{P}$ is linear. Then
\begin{align*}
(\hat{P}\Psi,iH\hat{P}\Psi) &= (\hat{P}\Psi,\hat{P} iH\Psi) \text{ from \ref{eq:SM:1}} \\ 
&= (\hat{P}\Psi,\hat{P} iE\Psi) \\
&= iE(\hat{P}\Psi,\hat{P}\Psi) \text{ as $\hat{P}$ linear} \\
&= iE 
\end{align*}

Now suppose $\hat{T}$ linear and complete as above giving
\[
(\hat{T}\Psi,iH\hat{T }\Psi) = -iE(\hat{T}\Psi,\hat{T}\Psi)
\]
Contradiction. 
Supposing instead $\hat{T}$ antilinear gives 
\[
(\hat{T}\Psi,iH\hat{T }\Psi) = iE(\hat{T}\Psi,\hat{T}\Psi)
\]
Hence must have $\hat{P}$ linear and unitary, whereas $\hat{T}$ antilinear and antiunitary. 
\end{proof}

%%%%%%%%%%%%%%%%%%%%%%%%%%%%%%%%%%%%%%%%%%%%%%%
\subsection{Parity}

\subsubsection*{Scalar fields}
\begin{definition}[Scalar Fields]
A complex scalar field is 
\[
\phi(x) = \sum_p \left[ a(p) e^{-ip\cdot x} + c^\dagger(p) e^{ip\cdot x} \right]
\]
\end{definition}
$\hat{P}: \ket{p} \to {\eta^a}^\ast \ket{p_P}$ where $p_P = (p^0,-\bm{p})$ and ${\eta^a}^\ast$ is a complex phase. For later define in analogy $x_P = (x^0, -\bm{x})$
\[
\Rightarrow \hat{P} a^\dagger (p) \ket{0} = {\eta^a}^\ast a^\dagger (p_P) \ket{0}
\]
since $\hat{P}\hat{P}^{-1}=I$ and assuming $\hat{P}\ket{0}=\ket{0}$
\[
\hat{P} a^\dagger (p) \hat{P}^{-1} = {\eta^a}^\ast a^\dagger (p_P)
\]
To conserve normalisation, $\hat{P} a(p) \hat{P}^{-1} = \eta^{a} a(p_P)$. Similarly $\hat{P} c^\dagger(p) \hat{P}^{-1} = {\eta^c}^\ast c^\dagger(p_P)$. Thus 
\begin{align*}
\hat{P} \phi(x) \hat{P}^{-1} &= \sum_p \left[ \hat{P} a(p) \hat{P}^{-1} e^{-ip.x} + \hat{P} c^\dagger(p) \hat{P}^{-1} e^{ip\cdot x} \right] \\ 
&= \sum_p \left[ \eta^a a(p_P) e^{-ip\cdot x} + {\eta^c}^\ast c^\dagger(p_P) e^{ip\cdot x} \right] \\
\text{Relabelling $p \leftrightarrow p_P$ } &= \sum_{p_P} \left[ \eta^a a(p) e^{-ip_P\cdot x} + {\eta^c}^\ast c^\dagger(p) e^{ip_P \cdot x} \right] \\
[p_P \cdot x = p\cdot x_P] \Rightarrow &= \sum_{p_P} \left[ \eta^a a(p) e^{-ip\cdot x_P} + {\eta^c}^\ast c^\dagger(p) e^{ip \cdot x_P} \right]  \\
[\sum_p = \sum_{p_P}] \Rightarrow &= \sum_{p} \left[ \eta^a a(p) e^{-ip\cdot x_P} + {\eta^c}^\ast c^\dagger(p) e^{ip \cdot x_P} \right] 
\end{align*}
This does not look like $\phi(x_P)$ unless $\eta^a = {\eta^c}^\ast \equiv \eta_P$ and otherwise would note in general find $\comm[\phi(x)]{\hat{P}\phi^\dagger(y) \hat{P}^{-1}}$ vanishes for spacelike $x-y_p$. Hence
\[
\hat{P} \phi(x) \hat{P}^{-1} = \eta_P \phi(x_P)
\]
\\
Note that for a real scalar field $a=c$ and so $\eta^a = {\eta^a}^\ast \Rightarrow \eta_P = \pm 1$. For a complex field, we may not have real $\eta_P$, but if there is some conserved charge we can redefine $\hat{P}$ such that $\eta_P = \pm1$

\subsubsection*{Vecotr fields}
\begin{definition}[Vector Fields]
A vector field is 
\[
V^\mu(x) = \sum_{p,\lambda} \left[ \eps^\mu(\lambda,p) a^\lambda(p) e^{-ip\cdot x} +{\eps^\mu}^\ast(\lambda,p) {c^\lambda}^\dagger(p) e^{ip\cdot x} \right]
\]
$\lambda = 0, \pm1$ is helicity, $\eps^\mu$ polarisation vectors. 
\end{definition}
Use $\eps^\mu(\lambda, p_P) = -\mbb{P}^\mu_\nu \eps^\nu (\lambda,p)$. In analogy to the above treatment we find 
\[
\hat{P} V^\mu(x) \hat{P}^{-1} = -\eta_P \mbb{P}^\mu_\nu V^\nu(x_P)
\]
Vectos have $\eta_P = -1$, axial vectors have $\eta_P = 1$. \\

\subsubsection*{Dirac Field}
For a Dirac field, creation/annihilation operators should behave like those for bosons. The 3-momentum reverses direction, the spin component s is changed. 
\eq{
\hat{P} b^s(p) \hat{P}^{-1} &= \eta^b b^s(p_P) \\
\hat{P} {d^s}^\dagger(p) \hat{P}^{-1} &= {\eta^d}^\dagger {d^s}^\dagger(p_P)
}
Then
\eq{
\hat{P}\psi(x)\hat{P}^{-1} &= \sum_{p,s} \left[ \eta^b b^s(p_P) u^s(p) e^{-ip\cdot x} + {\eta^d}^\ast {d^s}^\dagger(p_P) v^s(p) e^{ip\cdot x} \right] \\
&= \sum_{p,s} \left[ \eta^b b^s(p) u^s(p_P) e^{-ip\cdot x_P} + {\eta^d}^\ast {d^s}^\dagger(p) v^s(p_P) e^{ip\cdot x_P} \right]
}
One can verify
\eq{
u^s(p_P) &= \gamma^0 u^s(p) \\
v^s(p_P) &= -\gamma^0 v^s(p)
}
so 
\eq{
\hat{P}\psi(x) \hat{P}^{-1} = \sum_{p,s} \left[ \eta^b b^s(p) \gamma^0 u^s(p) e^{-ip\cdot x_P} - {\eta^d}^\ast {d^s}^\dagger(p) \gamma^0 u^s(p) e^{ip\cdot x_P} \right]
}
Require $\eta^b = -{\eta^d}^\ast=\eta_P$ so that 
\eq{
\hat{P} \psi(X) \hat{P}^{-1} = \eta_P \gamma^0 \psi(x_P) \equiv \psi^P(x)
}
Then 
\[
\bar{\psi}^P(x) = \hat{P}\bar{\psi}(x) \hat{P}^{-1} = \eta_P^\ast \bar\psi(x_P) \gamma^0
\]
Note 
\begin{itemize}
    \item $\hat{P} \psi_L(x) \hat{P}^{-1} = \eta_P \gamma^0 \psi_R(x_P)$ 
    \item It can be checked that $\psi$ satisfies the Dirac equation $\Rightarrow \psi^P$ satisfies the Dirac equation.  
\end{itemize}
From the above we can determine the transformation properties of fermion bilinears. 
\eq{
\bar{\psi}(x) \psi(x) &\to \hat{P} \bar{\psi}(x) \hat{P}^{-1} \hat{P} \bar{\psi}(x) \hat{P}^{-1} = \bar{\psi}(x_P) \psi(x_P) \quad &\text{(scalar)} \\
\bar{\psi}(x) \gamma^5 \psi(x) &\to -\bar{\psi}(x_P) \gamma^5 \psi(x_P) \quad &\text{(pseudoscalar)} \\
\bar{\psi}(x) \gamma^\mu \psi(x) &\to \mbb{P}^\mu_\nu\bar{\psi}(x_P) \gamma^\nu \psi(x_P) \quad &\text{(vector)} \\
\bar{\psi}(x) \gamma^\mu \gamma^5 \psi(x) &\to  - \mbb{P}^\mu_\nu\bar{\psi}(x_P) \gamma^\nu  \gamma^5 \psi(x_P) \quad &\text{(axial vector)}
} 

%%%%%%%%%%%%%%%%%%%%%%%%%%%%%%
\subsection{Charge conjugation}
$\hat{C}$ is a linear and unitary operator sending particles $\leftrightarrow$ antiparticles 

\subsubsection*{Scalar Field}
Lorentz symmetry constrains the phases 
\eq{
\hat{C} a(p) \hat{C}^{-1} &= \eta_C c(p) \\
\hat{C} c(p) \hat{C}^{-1} &= {\eta_C}^\ast a(p)
}
Then 
\eq{
\hat{C} \ket{particle, p} &= \hat{C}a^\dagger(p) \ket{0} \\
&= {\eta_C}^\ast c^\dagger(p) \ket{0} \\
&= {\eta_C}^\ast \ket{antiparticle,p}
}
From the decomposition 
\eq{
\hat{C}\phi(x) \hat{C}^{-1} = \eta_C \phi^\dagger (x) \\
\hat{C}\phi^\dagger(x) \hat{C}^{-1} = {\eta_C}^\ast \phi(x)
}
For a real scalar field $\phi=\phi^\dagger$ and so $\eta_C = \pm1$. 

\subsubsection*{Vector field}
Photon field must obey $\hat{C} A_\mu(x) \hat{C}^{-1} = -A_\mu (x)$. Hence a $\pi^0$ meson can decay to $2\gamma \Rightarrow \eta_C^{\pi^0} = (-1)^2 = 1$.
For a complex field, $\eta_C$ is arbitrary. Say $\eta_C= e^{2i\beta}$, we can do a global $U(1)$ transform st $\phi \to \phi^\prime = e^{-i\beta}\phi$ such that $\eta_C^\prime = 1$.

\subsubsection*{Dirac Field}
Define the matrix $C$ such that $(\gamma^\mu C)^T = \gamma^\mu C$. In the chiral basis where 
\eq{
{\gamma^0}^T &= \gamma^0 \\
{\gamma^1}^T &= -\gamma^1 \\
{\gamma^2}^T &= \gamma^2 \\
{\gamma^3}^T &= -\gamma^3 
}
a suitable choice is 
\eq{
C = =i\gamma^0 \gamma^2 = \begin{pmatrix} i\sigma^2 & 0 \\ 0 & -i\sigma^2 \end{pmatrix}
}
giving 
\[
C = -C^T = -C^\dagger = -C^{-1}
\]
Then 
\eq{
(\gamma^\mu)^T &= -C^{-1} \gamma^\mu C \\
{\gamma^5}^T &= C^{-1} \gamma^5 C
}
similarly to bosons 
\eq{
\hat{C} b^s(p) \hat{C}^{-1} &= \eta_C d^s(p) \\
\underbrace{\hat{C} {d^s}^\dagger(p) \hat{C}^{-1}}_{\text{in } \psi} &= \underbrace{\eta_C {b^s}^\dagger (p)}_{\text{in } \bar{\psi}}
}
Now consider 
\eq{
\hat{C} \psi(x) \hat{C}^{-1} = \eta_C \sum_{p,s} \left[ d^s(p) u^s(p) e^{-ip\cdot x} + {b^s}^\dagger v^s(p) e^{ip\cdot x} \right]
}
and compare with 
\eq{
{\bar{\psi}}^T (x) = \sum_{p,s} \left[ {b^s}^\dagger(p) {{\bar{u}}^s}^T (p) e^{ip\cdot x} + d^s {{\bar{v}}^s}^T (p) e^{-ip\cdot x} \right]
}
Consider the spinors and take $\eta^s = i\sigma^2 {\xi^s}^\ast$ (choosing a basis for the spinors) we can write 
\eq{
v^s(p) &= C {\bar{u}^s}^T \\
u^s(p) &= C {\bar{v}^s}^T \\
}
and so 
\eq{
\psi^C(x) = \hat{C} \psi(x) \hat{C}^{-1} = \eta_C C\bar{\psi}^T (x)
}
similarly 
\eq{
\bar{\psi}^C(x) = \hat{C} \bar{\psi}(x) \hat{C}^{-1} = {\eta_C}^\ast \psi^T (x) C = -{\eta_C}^\ast \psi^T(x) C^{-1}
}
Note that $\psi(x)$ satsifes the Dirac eqn $\Rightarrow \; \psi^C(x)$ does. 
\begin{itemize}
    \item Majorana fermions have $b^s(p) = d^s(p) \Rightarrow$ particle is its own anti particle. In this case $\psi = \psi^C$. 
    \item Is is note known whether the only neutral fermions in the SM (neutrinos) are Majorana (c.f. neutrinoless double beta decay). 
\end{itemize}

\subsubsection*{Fermion Bilinears}
Note it is important to keep track of what's an operator ($\hat{C}$) nad what is a matrix in spinor space ($C$). 
\begin{example}
\eq{
j^\mu(x) &= \bar{\psi}(x) \gamma^\mu \psi(x) \\ 
\Rightarrow \hat{C} j^\mu \hat{C}^{-1 } &= \hat{C}\bar{\psi} \hat{C}^{-1} \gamma^\mu \hat{C} \psi \hat{C}^{-1} \\
&= -\eta_C^\ast \eta_C \psi^T C^{-1} \gamma^\mu C \bar{\psi}^T  \\
&= - \psi_\alpha (C^{-1} \gamma^\mu C)_{\alpha\beta} \bar{\psi}_\beta \\
&= \bar{\psi}_\beta (C^{-1} \gamma^\mu C)_{\alpha\beta} \psi_\alpha \quad \text{(fermions anticommute)} \\
&= \bar{\psi}_\beta (C^{-1} \gamma^\mu C)_{\beta\alpha}^T \psi_\alpha \\
&= \bar{\psi} (C^{-1} \gamma^\mu C)^T \psi \\
&= -\bar{\psi} \gamma^\mu \psi = -j^\mu
}
Similarly 
\eq{
\hat{C} {j^\mu}^5 \hat{C}^{-1} = {j^\mu}^5
}
where ${j^\mu}^5 = \bar{\psi} \gamma^\mu \gamma^5 \psi$.
\end{example}

%%%%%%%%%%%%%%%%%%%%%%%%%%%%%%%%%%%%%%%%%%%%%%%%%%%%%%%%%%%%
\subsection{Time Reversal}
Take the notation $x^\mu_T = (-x^0, \bm{x})$, $p^\mu_T = (p^0, -\bm{p})$. In T-symmetric theories, the physics is unchanged if time runs backwards. 

\subsubsection*{Boson Field}
\eq{
\hat{T} a(p) \hat{T}^{-1} &= \eta_T a(p_T) \\
\hat{T} c^\dagger(p) \hat{T}^{-1} &= \eta_T c^\dagger (p_T)
}
From the decomposition, recalling $\hat{T}$ antihermitian, 
\eq{
\hat{T} \phi(x) \hat{T}^{-1} &= \sum_p \left[ \hat{T} a(p) \hat{T}^{-1} e^{ip\cdot x} + \hat{T} c^\dagger (p) \hat{T}^{-1} e^{-ip\cdot x} \right] 
}
So using $p_T \cdot x  = -p\cdot x_T$ 
\eq{
\hat{T} \phi(x) \hat{T}^{-1} &= \eta_T \sum_p \left[ a(p) e^{-p\cdot x_T} + c^T(p) e^{ip\cdot x_T} \right]
}
\subsubsection*{Dirac Field}
$\hat{T}$ flips sign of any momentum. The creation/annihilation ops can be taken to transform as 
\eq{
\hat{T} b^s(p) \hat{T}^{-1} & = \eta_T (-1)^{\frac{1}{2}-s} b^{-s} (p_T) \\
\hat{T} {d^s}^\dagger(p) \hat{T}^{-1} & = \eta_T (-1)^{\frac{1}{2}-s} {d^{-s}}^\dagger (p_T)
}
It can be shown that 
\eq{
(-1)^{\frac{1}{2}-s} {u^{-s}}^\ast (p_T) &= -Bu^s(p) \\
(-1)^{\frac{1}{2}-s} {v^{-s}}^\ast (p_T) &= -Bv^s(p) 
}
where 
\eq{
B = C^{-1} \gamma^5 = \begin{pmatrix} i\sigma^2 & 0 \\ 0 & i\sigma^2 \end{pmatrix}
}
Then 
\eq{
\hat{T} \psi(x) \hat{T}^{-1} &= \eta_T \sum_{p,s} (-1)^{\frac{1}{2}-s} \left[ b^{-s}(p_T) {u^s}^\ast(p) e^{ip\cdot x} + {d^{-s}}^\dagger(p_T) {v^s}^\ast(p) e^{-ip\cdot x}   \right] \\
&= \eta_T \sum_{p,s} (-1)^{\frac{1}{2}-s+1} \left[ b^{s}(p) {u^{-s}}^\ast(p_T) e^{ip\cdot x_T} + {d^{s}}^\dagger(p) {v^{-s}}^\ast(p_T) e^{ip\cdot x_T}   \right] \\
&= \eta_T B \psi(x_T)
}
Similarly 
\eq{
\hat{T} \bar{\psi}(x) \hat{T}^{-1} = \eta_T^\ast \bar{\psi}(x_T) B^{-1}
}
Then some bilinears we have 
\eq{
\hat{T} \bar{\psi}(x) \psi(x) \hat{T}^{-1} &= \bar{\psi}(x_T) \psi(x_T) \\
\hat{T} \bar{\psi}(x) \gamma^\mu \psi(x) \hat{T}^{-1} &= \bar{\psi}(x_T) B^{-1} {\gamma^\mu}^\ast B \psi(x_T)
}
Now we can check 
\eq{
B^{-1} {\gamma^0}^\ast B &= \gamma^0 \\
B^{-1} {\gamma^0i}^\ast B &= -\gamma^i \\ 
\Rightarrow B^{-1} {\gamma^\mu}^\ast B &= -\mbb{T}^\mu_\nu \gamma^\nu
}

%%%%%%%%%%%%%%%%%%%%%%%%%%%%%%%%%%%%%%%%%%%%
\subsection{Scattering S-Matrix}
Define 
\eq{
\braket{p_1,p_2,\dots| S | k_A, k_B, \dots} &= \tensor[_o]{\braket{p_1,p_2,\dots| k_A, k_B, \dots}}{_i} \\
&= \lim_{T\to\infty} \braket{p_1,p_2,\dots | Te^{-i\int_{-T}^T V(t) dt} | k_A, k_B, \dots}
}
with 
\eq{
V(t) = -\int d^3 x \mc{L}_I
}
the potential energy term. 
\begin{example}
In QED 
\eq{
\mc{L}_I = -e \bar{\psi} \gamma^\mu A_\mu \psi
}
\end{example}
Now we have the table of transformations 
\begin{center}$
\begin{array}{cccc}
    \text{Quantity} & \hat{P}\cdot\hat{P}^{-1} & \hat{C}\cdot\hat{C}^{-1} & \hat{T}\cdot\hat{T}^{-1} \\
    \hline
    \hline
    \mc{L}_I(x) & \mc{L}_I(x_P) & \mc{L}_I(x) & \mc{L}_I(x_T) \\
    V(t) & V(t) & V(t) & V(-t) \\
    S & ? & ? & ? \\
\end{array}
$\end{center}

Now write 
\eq{
S = \sum_{n=0}^\infty (-i)^n \int_{-\infty}^\infty dt_1 \int_{-\infty}^{t_1} dt_2 \dots \int_{-\infty}^{t_{n-1}} dt_n V(t_1) V(t_2) \dots V(t_n) \\
\Rightarrow S_T \ \hat{T} S \hat{T}^{-1} =  \sum_{n=0}^\infty (i)^n \int_{-\infty}^\infty dt_1 \int_{-\infty}^{t_1} dt_2 \dots \int_{-\infty}^{t_{n-1}} dt_n V(-t_1) V(-t_2) \dots V(-t_n)
}
Substituting $\tau = -t_{n+1-i}$ 
\eq{
S_T &= \sum_{n=0}^\infty (i)^n \int_\infty^{-\infty} (-d\tau_n) \int_\infty^{-t_1} (-d\tau_{n-1}) \dots \int_\infty^{-t_{n-1}} (-d\tau_1) V(\tau_n) V(\tau_{n-1})\dots V(\tau_1) \\
&=\sum_{n=0}^\infty (i)^n \int_{-\infty}^\infty d\tau_n \int_{-t_1}^\infty d\tau_{n-1} \dots \int_{-t_{n-1}}^\infty d\tau_1 V(\tau_n) V(\tau_{n-1})\dots V(\tau_1) \\ 
&= \sum_{n=0}^\infty (i)^n \int_{-\infty}^\infty d\tau_n \int_{\tau_n}^\infty d\tau_{n-1} \dots \int_{\tau_2}^\infty d\tau_1 V(\tau_n) V(\tau_{n-1})\dots V(\tau_1)
}
Geometrically it can be seen 
\eq{
\int_{-\infty}^\infty d\tau_n \int_{\tau_n}^\infty d\tau_{n-1} = \int_{-\infty}^\infty d\tau_{n-1} \int_{-\infty}^{\tau_{n-1}} d\tau_n 
}
so successively swapping 
\eq{
S_T = \sum_{n=0}^\infty (i)^n \int_{-\infty}^\infty d\tau_1 \int_{-\infty}^{\tau_1} d\tau_2 \dots \int_{-\infty}^{\tau_{n-1}} d\tau_n V(\tau_n) V(\tau_{n-1})\dots V(\tau_1)
}
Now consider 
\eq{
S^\dagger &= \sum_{n=0}^\infty (i)^n \int_{-\infty}^\infty dt_1 \int_{-\infty}^{t_1} dt_2 \dots \int_{-\infty}^{t_{n-1}} dt_n [V(t_1) V(t_2) \dots V(t_n)]^\dagger \\
&= \sum_{n=0}^\infty (i)^n \int_{-\infty}^\infty dt_1 \int_{-\infty}^{t_1} dt_2 \dots \int_{-\infty}^{t_{n-1}} dt_n V(t_n) V(t_{n-1}) \dots V(t_1)
}
So we have shown 
\eq{
S_T = S^\dagger
}
Hence note ${S_T}^\dagger = S$. Now consider $\ket{\xi},\ket{\eta}$ with 
\eq{
\ket{\xi_T} &= \hat{T} \ket{\xi} \\
\ket{\eta_T} &= \hat{T} \ket{\eta}
}

 \end{document} 